

## 1. THE SPSA “PROCESS”

We analyze the SPSA algorithm in 1 dimension as implemented in fishtest.  $w, d, l$  denote respectively the win, draw and loss ratio. We use the Bayes Elo model. I.e. we have for  $\beta = \log(10)/400$

$$w = \frac{1}{1 + e^{-\beta(x-\delta)}}$$

$$l = \frac{1}{1 + e^{-\beta(-x-\delta)}}$$

where  $\delta$  is the drawelo parameter. We score an engine game by  $\pm 1, 0, -1$  for respectively a win, draw, loss. We assume that  $x$  is small. We have for  $E = e^{\beta\delta}$ .

$$w = \frac{1}{1 + Ee^{-\beta x}}$$

$$\cong \frac{1}{1 + E(1 - \beta x)}$$

$$= \frac{1}{1 + E} \left( 1 + \frac{\beta x}{1 + E} \right)$$

$$= \frac{1}{1 + E} + \frac{\beta x E}{(1 + E)^2}$$

and similarly

$$l = \frac{1}{1 + E} - \frac{\beta x E}{(1 + E)^2}$$

Hence the expected score and its standard deviation are respectively given by

$$\mu = w - l$$

$$\cong \frac{2\beta x E}{(1 + E)^2}$$

$$\sigma = \sqrt{w + l - (w - l)^2}$$

$$\cong \sqrt{\frac{2}{1 + E}}$$

Let  $p$  be an engine parameter and let  $f(p)$  be the function that maps  $p$  to Bayes Elo. We play a match of  $p + c$  against  $p - c$  and replace  $p$  by<sup>1</sup>

$$\begin{cases} p + \frac{a}{c} & \text{in case of a win} \\ p & \text{in case of a draw} \\ p - \frac{a}{c} & \text{in case of a loss} \end{cases}$$

So we can think of the dynamics of  $p$  as a discrete version of the continuous process

$$dp = \frac{a}{c}(\mu dt + \sigma dW_t)$$

where  $(\mu, \sigma)$  are the mean and standard deviation of a single game and  $W_t$  is a Wiener process. Using the approximation

$$x = f(p + c) - f(p - c) = 2cf'(p)$$

---

<sup>1</sup>We see that  $a$  is the learning rate. Using  $a/2c$  would be somewhat more natural.

2

we find

$$dp = \frac{a}{c} \left( \frac{4\beta c f'(p) E}{(1+E)^2} dt + \sqrt{\frac{2}{1+E}} dW_t \right)$$

Hence

$$dp = \frac{4\beta a E}{(1+E)^2} f'(p) dt + \frac{a}{c} \sqrt{\frac{2}{1+E}} dW_t$$

which we will write as

$$dp = u_1 a f'(p) dt + u_2 \frac{a}{c} dW_t$$

with

$$u_1 = \frac{4\beta E}{(1+E)^2}$$

$$u_2 = \sqrt{\frac{2}{1+E}}$$

**Example 1.1.** Assume  $\delta = 220$  (a realistic value for self testing at short time controls). Then we find

$$u_1 = 0.003950$$

$$u_2 = 0.6631$$

In the special case that

$$(1) \quad f(p) = -\xi(p - p_0)^2$$

$$dp = -2u_1 a \xi (p - p_0) dt + u_2 dW_t$$

If  $a, c$  are constant then this is an Ornstein-Uhlenbeck process

$$dp = -\theta(p - \mu) dt + \sigma dW_t$$

with

$$\mu = p_0$$

$$\theta = 2u_1 a \xi$$

$$\sigma = u_2 \frac{a}{c}$$

*Remark 1.2.* The parameters in an Ornstein-Uhlenbeck process are actually just location and scaling parameters for  $p$  and  $t$ . Replacing  $p$  by  $p - \mu$  we may assume  $\mu = 0$ . Putting  $t = \theta^{-1}s$ ,  $p = \sigma\theta^{-1/2}q$  and using that  $W_{\theta s} = \theta^{1/2}W_s$  we end up with the equation

$$dq = -q ds + dW_s$$

We deduce that

$$\theta^{-1} = \frac{1}{2u_1 \xi a}$$

acts like a natural time scale and that

$$\frac{\sigma}{\sqrt{\theta}} = \frac{u_2}{\sqrt{2u_1 \xi}} \frac{\sqrt{a}}{c}$$

is a natural scale for the range of the parameter  $p$  in SPSA.

## 2. SOLVING A CASE WITH VARYING HYPERPARAMETERS

Now we consider the case where  $f$  is quadratic as in (1) and  $a = a(t)$ ,  $c = c(t)$  are time dependent via

$$a(t) = \frac{a_0}{(A+t)^\alpha}$$

$$c(t) = \frac{c_0}{t^\gamma}$$

It is clear that without loss of generality we may assume  $p_0 = 0$ . We have to solve

$$dp = -2\xi u_1 \frac{a_0}{(A+t)^\alpha} p dt + u_2 \frac{a_0}{c_0} \frac{t^\gamma}{(A+t)^\alpha} dW_t$$

We consider first the unperturbed system

$$dp = -2\xi u_1 \frac{a_0}{(A+t)^\alpha} p dt$$

It can be rewritten as

$$d \log p = -\frac{2\xi u_1 a_0}{1-\alpha} d(A+t)^{1-\alpha}$$

so that we get

$$p = C \exp\left(-\frac{2\xi u_1 a_0}{1-\alpha} (A+t)^{1-\alpha}\right)$$

We now find a particular solution of the perturbed system using variation of constants. We get

$$\exp\left(-\frac{2\xi u_1 a_0}{1-\alpha} (A+t)^{1-\alpha}\right) dC = u_2 \frac{a_0}{c_0} \frac{t^\gamma}{(A+t)^\alpha} dW_t$$

so that we may as a particular solution we may take

$$u_2 \frac{a_0}{c_0} \exp\left(-\frac{2\xi u_1 a_0}{1-\alpha} (A+t)^{1-\alpha}\right) \int_0^t \exp\left(\frac{2\xi u_1 a_0}{1-\alpha} (A+s)^{1-\alpha}\right) \frac{s^\gamma}{(A+s)^\alpha} dW_s$$

and the full solution is given by

$$\exp\left(-\frac{2\xi u_1 a_0}{1-\alpha} (A+t)^{1-\alpha}\right) \left(C + u_2 \frac{a_0}{c_0} \int_0^t \exp\left(\frac{2\xi u_1 a_0}{1-\alpha} (A+s)^{1-\alpha}\right) \frac{s^\gamma}{(A+s)^\alpha} dW_s\right)$$

It follows that at a time  $t$  we have  $p \sim N(\mu_t, \sigma_t^2)$  with

$$\mu_t = C \exp\left(-\frac{2\xi u_1 a_0}{1-\alpha}(A+t)^{1-\alpha}\right)$$

$$\sigma_t = u_2 \frac{a_0}{c_0} \exp\left(-\frac{2\xi u_1 a_0}{1-\alpha}(A+t)^{1-\alpha}\right) \sqrt{\int_0^t \exp\left(\frac{4\xi u_1 a_0}{1-\alpha}(A+s)^{1-\alpha}\right) \frac{s^{2\gamma}}{(A+s)^{2\alpha}} ds}$$

Let us now investigate the asymptotic behaviour of the intergral under the square root sign. Put

$$r = (A+s)^{1-\alpha}$$

so that

$$\begin{aligned} dr &= (1-\alpha)(A+s)^{-\alpha} ds \\ &= (1-\alpha)r^{-\alpha/(1-\alpha)} ds \end{aligned}$$

and hence

$$ds = \frac{1}{1-\alpha} r^{\alpha/(1-\alpha)} dr$$

We obtain

$$\int_0^t \exp\left(\frac{4\xi u_1 a_0}{1-\alpha}(A+s)^{1-\alpha}\right) \frac{s^{2\gamma}}{(A+s)^{2\alpha}} ds = \frac{1}{1-\alpha} \int_{A^{1-\alpha}}^{(A+t)^{1-\alpha}} \exp\left(\frac{4\xi u_1 a_0}{1-\alpha} r\right) \frac{(r^{1/(1-\alpha)} - A)^{2\gamma}}{r^{\alpha/(1-\alpha)}} dr$$

So it seems that we have to understand the asymptotic behaviour of

$$\int_{K_0}^K e^{r-K} r^{-\psi} dr = \int_0^{K-K_0} \frac{e^{-r}}{(K-r)^\psi} dr$$

for  $K \rightarrow \infty$ , where  $\psi = (\alpha - 2\gamma)/(1 - \alpha)$  which in the case of fishtest ( $\alpha = 0.602$ ,  $\gamma = 0.101$  is slightly bigger 1).